Misc/MonadEquiv.v
@@ -18,6 +18,24 @@ Require Import HSLib.MonadComp.Monad.
 Include HSLib.MonadComp.Monad.
 End Comp.
 
+Axiom fmap_ret :
+  forall (M : Type -> Type) (inst : Join.Monad M) (A B : Type) (f : A -> B)
+    (x : A), fmap f (Join.ret x) = Join.ret (f x).
+
+Axiom join_ret :
+  forall (M : Type -> Type) (inst : Join.Monad M) (X : Type) (mx : M X),
+    Join.join (Join.ret mx) = mx.
+
+Axiom fmap_join :
+  forall (M : Type -> Type) (inst : Join.Monad M) (A B : Type) (f : A -> B)
+    (x : M (M A)),
+      fmap f (Join.join x) = Join.join (fmap (fmap f) x).
+
+Axiom fmap_pres_comp' :
+  forall (M : Type -> Type) (inst : Join.Monad M) (A B C : Type)
+  (f : A -> B) (g : B -> C) (x : M A),
+    fmap (fun x : A => g (f x)) x = fmap g (fmap f x).
+
 Instance JoinToBind (M : Type -> Type) (inst : Join.Monad M) : Bind.Monad M :=
 {
     is_functor := @Join.is_functor M inst;
@@ -26,20 +44,12 @@ Instance JoinToBind (M : Type -> Type) (inst : Join.Monad M) : Bind.Monad M :=
         (fmap f .> Join.join) ma
 }.
 Proof.
-(*  Focus 2. intros. Print Join.Monad. unfold compose.*)
-  intros.
-  unfold compose.
-  Print Join.Monad.
-  assert (H := Join.join_law).
-  specialize (H A). unfold compose in H.
-  Print Applicative.
-  Print Functor.
-  Search Join.join.
-  Search Join.ret.
-  cut (fmap f (Join.ret a) = Join.ret (f a)).
-    intros ->.
-    Focus 2.
-
+  all: intros.
+    unfold compose. rewrite fmap_ret, join_ret. reflexivity.
+    rewrite <- Join.ret_law. unfold compose. rewrite join_ret. reflexivity.
+    Focus 2. rewrite fmap_ret. reflexivity.
+    Focus 2. unfold compose. rewrite <- fmap_pres_comp'. reflexivity.
+    unfold compose. rewrite fmap_join, <- ?fmap_pres_comp'.
 Abort.
 
 Instance BindToComp (M : Type -> Type) (inst : Bind.Monad M)
@@ -51,10 +61,11 @@ Instance BindToComp (M : Type -> Type) (inst : Bind.Monad M)
         fun a : A => Bind.bind (f a) g
 }.
 Proof.
-  all: intros; extensionality x.
+  all: intros; try ext x.
     rewrite Bind.assoc. reflexivity.
     apply Bind.id_left.
     apply Bind.id_right.
+    apply Bind.fmap_ret.
 Defined.
 
 Instance BindToJoin (M : Type -> Type) (inst : Bind.Monad M)
@@ -66,8 +77,25 @@ Instance BindToJoin (M : Type -> Type) (inst : Bind.Monad M)
         Bind.bind x id
 }.
 Proof.
-  intros. unfold compose. extensionality x.
-    rewrite Bind.assoc.
-  Focus 2. intros. Print Bind.Monad. unfold compose.
-    extensionality x. rewrite Bind.id_left.
+  intros. unfold compose. ext x. rewrite Bind.assoc, Bind.bind_fmap.
+    unfold compose, id. reflexivity.
+  intros. unfold compose. ext x. rewrite Bind.id_left, Bind.bind_fmap.
+    unfold compose, id. rewrite Bind.id_right. reflexivity.
+  intros. unfold compose, id. ext x. rewrite Bind.id_left. reflexivity.
+  intros. rewrite Bind.fmap_ret. reflexivity.
+Defined.
+
+Instance CompToBind (M : Type -> Type) (inst : Comp.Monad M)
+  : Bind.Monad M :=
+{
+    is_functor := @Comp.is_functor M inst;
+    ret := @Comp.ret M inst;
+    bind := fun (A B : Type) (ma : M A) (f : A -> M B) =>
+      Comp.compM id f ma
+}.
+Proof.
+  all: intros.
+    Focus 2. rewrite Comp.id_right. reflexivity.
+    Focus 3. rewrite Comp.fmap_ret. reflexivity.
+    Focus 3. unfold compose, id. 
 Abort.
